\section*{Introducing the actors: matrices}
\gotosection{1}{2}

\newenvironment{xmatrix}{\begin{bmatrix*}[r]}{\end{bmatrix*}}

\begin{exercise}{2}
  \begin{enumerate}
    \item $\begin{xmatrix}1 & 2 & 3 \\ 4 & 5 & 6\end{xmatrix}
           \begin{xmatrix}7 & 8 \\ 9 & 0 \\ 1 & 2\end{xmatrix} =
           \begin{xmatrix}
              7 + 18 + 3 &  8 + 0 +  4 \\
             28 + 45 + 6 & 32 + 0 + 12
           \end{xmatrix} =
           \begin{xmatrix}28 & 12 \\ 79 & 44\end{xmatrix}$

    \item Incompatible matrices: the first matrix has 2 columns while the second
          one has 3 rows.

    \item $\begin{aligned}[t]
            \begin{xmatrix}
               1 & -1 &  1 \\
              -1 &  0 &  2 \\
              -1 &  1 &  1
            \end{xmatrix}
            \begin{xmatrix}
               0 &  1 & -1 \\
              -1 &  1 &  2 \\
               2 &  0 & -2
            \end{xmatrix} &=
            \begin{xmatrix}
              0 + 1 + 2 &  1 - 1 + 0 & -1 - 2 - 2 \\
              0 + 0 + 4 & -1 + 0 + 0 &  1 + 0 - 4 \\
              0 - 1 + 2 & -1 + 1 + 0 &  1 + 2 - 2
            \end{xmatrix} \\ &=
            \begin{xmatrix}
              3 &  0 & -5 \\
              4 & -1 & -3 \\
              1 &  0 &  1
            \end{xmatrix}
          \end{aligned}$

    \item $\begin{xmatrix}7 & 1 \\ -1 & 0 \\ 2 & 3\end{xmatrix}
           \begin{xmatrix}5 \\ -4\end{xmatrix} =
           \begin{xmatrix}
             35 - 4 \\
             -5 + 0 \\
             10 - 12
           \end{xmatrix} =
           \begin{xmatrix}31 \\ -5 \\ -2\end{xmatrix}$

    \item \def \tmp{\begin{bmatrix*}[r]0 & 1 \\ -1 & 3\end{bmatrix*}}
          $\begin{aligned}[t]
            \begin{xmatrix}1 & 2 \\ 0 & 3\end{xmatrix}
            \begin{xmatrix}1 & 4 \\ 1 & 3\end{xmatrix}
            \tmp &=
            \begin{xmatrix}
              1 + 2 & 4 + 6 \\
              0 + 3 & 0 + 9
            \end{xmatrix}
            \tmp \\ &=
            \begin{xmatrix}3 & 10 \\ 3 & 9\end{xmatrix}
            \tmp \\ &=
            \begin{xmatrix}
              0 + 3 &   0 +  9 \\
              -3 + 9 & -10 + 27
            \end{xmatrix} \\
            &= \begin{xmatrix}3 & 9 \\ 6 & 17\end{xmatrix}
          \end{aligned}$

    \item Incompatible matrices: the first matrix has 3 columns while the second
          one has 2 rows.
  \end{enumerate}
\end{exercise}

\begin{exercise}{3}
  \begin{enumerate}
    \item $\begin{pmatrix}AB_{13}\\AB_{23}\end{pmatrix} =
           \begin{xmatrix}1 & 2 & 0\\3 & 1 & -1\end{xmatrix}
           \begin{pmatrix}1 \\ 2 \\ 3\end{pmatrix} =
           \begin{pmatrix}1+4 \\ 3+2-3\end{pmatrix} =
           \begin{pmatrix}5 \\ 2\end{pmatrix}$
    \item $\begin{aligned}[t]
            \begin{xmatrix}AB_{21} & AB_{22} & AB_{23}\end{xmatrix} &=
            \begin{xmatrix}3 & 1 & -1\end{xmatrix}
            \begin{xmatrix}
              2 & 5 & 1 \\
              1 & 4 & 2 \\
              1 & 3 & 3
            \end{xmatrix}
            \\ &=
            \begin{xmatrix}6 + 1 - 1 & 15 + 4 - 3 & 3 + 2 - 3\end{xmatrix}
            \\ &=
            \begin{xmatrix}6 & 16 & 2\end{xmatrix}
          \end{aligned}$
  \end{enumerate}
\end{exercise}

\begin{exercise}{5}
  Since $A$ is symmetric, $A = A^{\top}$.
  
  \begin{enumerate}
    \item True. $B^{\top}A = B^{\top}A^{\top} = (AB)^{\top}$ \QED
    \item True. $B^{\top}A^{\top} = (AB)^{\top} = (A^{\top}B)^{\top}$ \QED
    \item False. $(A^{\top}B)^{\top} = B^{\top}A \neq BA$, 
          since $B^{\top} = B$ doesn't hold if $B$ is not symmetric.
    \item False. $(AB)^{\top} = B^{\top}A^{\top} \neq A^{\top}B^{\top}$, 
          since $XY = YX$ iff $X$ is the inverse of $Y$.
  \end{enumerate}
\end{exercise}

\begin{exercise}{8}
  The only value of $a$ such that $AB = BA$ is $0$, as:
  \medskip

  $AB = \begin{xmatrix}1 & 1 \\ 1 & 0\end{xmatrix}
        \begin{xmatrix}1 & 0 \\ a & 1\end{xmatrix}
      = \begin{xmatrix}1 + a & 1 \\ 1 & 0\end{xmatrix}$
  \medskip

  $AB = \begin{xmatrix}1 & 0 \\ a & 1\end{xmatrix}
        \begin{xmatrix}1 & 1 \\ 1 & 0\end{xmatrix}
      = \begin{xmatrix}1 & 1 \\ 1 + a & a\end{xmatrix}$
  \medskip

  $\left\{
    \begin{aligned}
      1 + a &= 1 \\
          a &= 0
    \end{aligned}
  \right.\quad \Longrightarrow \quad a = 0$
\end{exercise}

\begin{exercise}{10}
  Follow the formula for the inverse of $2\times2$-matrix:

  \begin{align*}
    A^{-1} &= \frac{1}{a^2-0}\begin{xmatrix}a & -b\\0 & a\end{xmatrix} \\
           &= \begin{xmatrix}
                \frac{1}{a} & -\frac{b}{a} \\
                          0 &  \frac{1}{a}
              \end{xmatrix}
  \end{align*}
\end{exercise}

\begin{exercise}{15}
  Let $A = \begin{xmatrix}
             1 & a & b \\
             0 & 1 & c \\
             0 & 0 & 1
           \end{xmatrix}$,
  and $B = \begin{xmatrix}
             1 & x & y \\
             0 & 1 & z \\
             0 & 0 & 1
           \end{xmatrix}$.
  The product is
  
  $$AB =
    \begin{xmatrix}
      1 & x + a & y + az + b \\
      0 &     1 &      z + c \\
      0 &     0 &          1
    \end{xmatrix} =
    I_3 = \begin{xmatrix}1&0&0\\0&1&0\\0&0&1\end{xmatrix}$$
  
  Then we have:
  \medskip
  
  $\left\{
    \begin{aligned}
           x + a &= 0 \\
      y + az + b &= 0 \\
           z + c &= 0
    \end{aligned}
  \right.\quad \Longrightarrow \quad
  \left\{
    \begin{aligned}
               x &= -a \\
               z &= -c \\
      y - ac + b &= 0
    \end{aligned}
  \right.\quad \Longrightarrow \quad
  \left\{
    \begin{aligned}
      x &= -a     \\
      y &= ac - b \\
      z &= -c
    \end{aligned}
  \right.$
\end{exercise}

\begin{exercise}{16}
  From the definition of transpose and symmetric matrix,
  it is obvious that $(A^{\top})^{\top} = A$,
  and that if $A = A^{\top}$, then $A$ is symmetric.

  For any matrix $A$, since $(A^{\top}A)^{\top} = A^{\top}(A^{\top})^{\top} = A^{\top}A$,
  namely $A^{\top}A$ equal to its transpose, $A^{\top}A$ is symmetric. \QED
\end{exercise}
