\gotosection{1}{3}
\subsection{Linear transformations}

\begin{exercise}{4}
  \begin{enumerate}
    \item $T = \begin{xmatrix}
                 2 & 0 & 0 \\
                 0 & 1 & 0 \\
                 0 & 0 & 1
               \end{xmatrix}$

    \item $T = \begin{xmatrix}
                 0 & 1 & 0 \\
                 1 & 2 & 0 \\
                 1 & 0 & 1
               \end{xmatrix}$
  \end{enumerate}
\end{exercise}

\begin{exercise}{8}
  The $i$th column of $[T]$ is $T(\Vect{e}_i)$.

  \begin{enumerate}
    \item For \FunSS{T}{\mathbb{R}^5}{\mathbb{R}^6}, $[T]$ has 5 columns. Therefore,
          5 questions need answered, and they are $T(\Vect{e}_1), \hdots, T(\Vect{e}_5)$.

    \item For \FunSS{T}{\mathbb{R}^6}{\mathbb{R}^5}, $[T]$ has 6 columns. Therefore,
          6 questions need answered, and they are $T(\Vect{e}_1), \hdots, T(\Vect{e}_6)$.

    \item There are infinite answers. For instance, one can ask $T(2\Vect{e}_1), \hdots, T(2\Vect{e}_6)$.
          Then instead of $T$, one will get the columns of $2T$. However, if one
          multiplies the results with $\frac{1}{2}$, he or she can still get the
          original matrix $T$.
  \end{enumerate}
\end{exercise}

\begin{exercise}{9}
  Suppose $T$ is linear. Due to the linearity:

  \begin{align*}
    T(\begin{xmatrix}2 \\ -1 \\ 4\end{xmatrix})
      &= T(2\Vect{e}_1 - \Vect{e}_2 + 4\Vect{e}_3) \\
      &= 2T(\Vect{e}_1) - T(\Vect{e}_2) + 4T(\Vect{e}_3) \\
      &= 2\begin{xmatrix}2 \\ 1 \\ 1\end{xmatrix} -
          \begin{xmatrix}1 \\ 2 \\ 1\end{xmatrix} +
         4\begin{xmatrix}1 \\ 0 \\ 1\end{xmatrix} =
          \begin{xmatrix}7 \\ 0 \\ 5\end{xmatrix}
      \neq\begin{xmatrix}7 \\ 0 \\ 4\end{xmatrix}
  \end{align*}

  Therefore $T$ is not linear.
\end{exercise}

\begin{exercise}{13}
  \begin{enumerate}
    \item Nonsense.
    \item \FunSS{C \circ B}{\mathbb{R}^m}{\mathbb{R}^n}
    \item \FunSS{A \circ C}{\mathbb{R}^k}{\mathbb{R}^m}
    \item \FunSS{B \circ A \circ C}{\mathbb{R}^k}{\mathbb{R}^k}
    \item Nonsense.
    \item Nonsense.
    \item \FunSS{B \circ A}{\mathbb{R}^n}{\mathbb{R}^k}
    \item \FunSS{A \circ C \circ B}{\mathbb{R}^m}{\mathbb{R}^k}
    \item \FunSS{C \circ B \circ A}{\mathbb{R}^n}{\mathbb{R}^n}
    \item Nonsense.
  \end{enumerate}
\end{exercise}

\begin{exercise}{18}
  All sketches are hand-drawn in the separate sketch paper.
\end{exercise}

\begin{exercise}{19}
  \begin{enumerate}
    \item Let $A * B$ be the \textit{Jordan product} of $A$ and $B$. Since matrix addition is commutative, we have $A * B = \frac{AB + BA}{2} = \frac{BA + AB}{2} = B * A$. Hence the product is commutative. \QED
    \item $\begin{aligned}[t]
        A * (B * C) &= \frac{1}{2}(A\frac{BC + CB}{2} + \frac{BC + CB}{2}A) \\
                            &= \frac{1}{4}(A(BC+CB) + (BC+CB)A) \\
                            &= \frac{1}{4}(ABC+ACB+BCA+CBA) \\
        (A * B) * C &= \frac{1}{4}(CAB+CBA+ABC+BAC)
      \end{aligned}$
      
      $A * (B * C) - (A * B) * C = \frac{1}{4}(ACB+BCA-CAB-BAC) \neq 0$.
      \footnote{For example, let
                $A = \begin{xmatrix}0&1\\1&0\end{xmatrix},
                B = \begin{xmatrix}0&1\\1&0\end{xmatrix},
                C = \begin{xmatrix}1&2\\3&4\end{xmatrix}$,
                $ACB+BCA-CAB-BAC = \begin{xmatrix}6&2\\-2&-6\end{xmatrix}$.}
      Hence the two products are not equal, and the product is not associative. \QED
  \end{enumerate}
\end{exercise}

\begin{exercise}{20}
  For any $x = a_1+ib_1, y = a_2+ib_2$, and real numbers $m, n$.
  \def \Re{\mathrm{Re}}
  \def \C{c}
  \def \Mw{m_w}
  
  \begin{enumerate}
    \item $\begin{aligned}[t]
            \Re(mx+ny) &= \Re(ma_1+mib_1+na_2+nib_2) \\
                       &= ma_1 + na_2 = m\Re(a_1+ib_1) + n\Re(a_2 + ib_2) \\
                       &= m\Re(x) + n\Re(y)
          \end{aligned}$
                       
          $[\Re] = \begin{xmatrix}1 & 0\end{xmatrix}$.
          
    \item $\begin{aligned}[t]
            \Im(mx+ny) &= \Im(ma_1+mib_1+na_2+nib_2) \\
                       &= mib_1 + nib_2 = m\Im(a_1+ib_1) + n\Im(a_2 + ib_2) \\
                       &= m\Im(x) + n\Im(y)
          \end{aligned}$
                       
          $[\Im] = \begin{xmatrix}0 & 1\end{xmatrix}$.
          
    \item $\begin{aligned}[t]
            \C(mx+ny) &= \C(ma_1+mib_1+na_2+nib_2) \\
                      &= ma_1-mib_1+na_2-nib_2 \\
                      &= m \cdot \C(a_1+ib_1)+n \cdot \C(a_2+ib_2) \\
                      &= m \cdot \C(x) + n \cdot \C(y)
          \end{aligned}$
          
          $[\C] = \begin{xmatrix}1 & 0 \\ 0 & -1\end{xmatrix}$.
          
    \item $\begin{aligned}[t]
            \Mw(mx+ny) &= \Mw(ma_1+mib_1+na_2+nib_2) \\
                       &= (u+iv)(ma_1+mib_1+na_2+nib_2) \\
                       &= m(u+iv)(a_1+ib_1) + n(u+iv)(a_2+ib_2) \\
                       &= m \cdot \Mw(a_1+ib_1) + n \cdot \Mw(a_2+ib_2) \\
                       &= m \cdot \Mw(x) + n \cdot \Mw(y)
          \end{aligned}$
          
          $[\Mw]\cdot \Vect{e}_1 = (u + iv) \cdot 1 
                                 = \begin{xmatrix}u\\v\end{xmatrix} \\$
          $[\Mw]\cdot \Vect{e}_2 = (u + iv) \cdot i = iu - v
                                 = \begin{xmatrix}-v\\u\end{xmatrix} \\$
          $[\Mw] = \begin{xmatrix}u & -v\\v & u\end{xmatrix}$
  \end{enumerate}
\end{exercise}
